rename and refine lemmas in Formula.v.

Formula.v
@@ -1,140 +1,158 @@
-Require Import Id.
 From Coq Require Import Bool.Bool.
-Export Id.
+From Coq Require Import Strings.String.
 Export Bool.Bool.
 
-(*alias*)
-Definition id := Id.id. (*Type of id*)
-Definition Id := Id.Id. (*Constructor of id*)
+(** Identifier of the var is implement with string. *)
+Inductive id : Type :=
+| Id (n : string).
 
-(*Definition of formula*)
+(** TODO*)
+Definition eqb_string (x y : string) : bool :=
+  if string_dec x y then true else false.
+
+(** Define the equality on id. *)
+Definition eqb_id  (i1 i2:id): bool :=
+  match i1 with
+  | Id x => match i2 with
+            | Id y => eqb_string x y (*use equality on string*)
+            end
+  end.
+
+(** Equality on Ids is decidable. *)
+Lemma id_eq_dec : forall a b : id, {a = b} + {a <> b}.
+Proof.
+  intros.
+  destruct a,b.
+  decide equality.
+  apply string_dec.
+Defined. (* TODO make defined, since we will unfold it*)
+
+(** Exercise 2.1 *)
+(** Define formula. *)
 Inductive form :=
 | var : id-> form
-| bool : bool ->form
+| bbool : bool ->form
 | land : form -> form -> form
 | lor : form -> form -> form
 | mapsto : form -> form -> form
 | not : form -> form.
 
 
-(*Definition of valuation*)
-Definition valuation := id -> Datatypes.bool.
+(** Define valuation of the formula. *)
+Definition valuation := id -> bool.
 Definition empty_valuation : valuation := fun x => false.
 Definition override (V : valuation) (x : id) (b : Datatypes.bool) : valuation :=
-  fun y => if beq_id x y then b else V y.
+  fun y => if eqb_id x y then b else V y.
 
-(*Interprete the formula with valuation*)
-Fixpoint interp (V : valuation) (p : form) : Datatypes.bool :=
+(** Exercise 2.3 *)
+(** Interprete the formula with valuation. *)
+Fixpoint interp (V : valuation) (p : form) : bool :=
   match p with
   | var i => (V i)
-  | bool b => b
+  | bbool b => b
   | land f1 f2 => andb (interp V f1) (interp V f2)
   | lor f1 f2 => orb (interp V f1) (interp V f2)
   | mapsto f1 f2 => orb  (negb (interp V f1)) (interp V f2)
   | not f => negb (interp V f)
   end.
 
+(** Exercise 2.2 *)
 Module Test_override.
  Definition x := (var (Id "x")).
  Definition y := (var (Id "y")).
 
  Check (land (lor x (not y)) (lor (not x) y) ).
  Check (mapsto (not y) (lor x y) ).
- Check (land (land x (not x)) (bool true)).
+ Check (land (land x (not x)) (bbool true)).
 
  Definition context := override (override empty_valuation (Id "x") false) (Id "y") true.
 
 End Test_override.
 
 
-Lemma land_interp_interp: forall p1 p2 V, interp V p1=true /\ interp V p2=true <-> interp V (land p1 p2)=true.
+(** 
+    Define a tactic that we use a lot.
+    For a bool equaltion as a && b = ture in the assumption, 
+    it can be splited into a = true and b = true
+ **)
+Ltac split_andb_ture H :=
+  symmetry in H;
+  apply andb_true_eq in H;
+destruct H as [H H0];
+  symmetry in  H,H0.
+
+(** 
+    Helper lemmas for interp, which define the equavalence between interperation of a formula and its sub-formula(s).
+    We can expend the interperation on a formula if it has sub-formula(s). 
+ **)
+
+Lemma split_interp_land: forall p1 p2 V, interp V p1=true /\ interp V p2=true <-> interp V (land p1 p2)=true.
 Proof.
-  intros.
-  split.
-  - intro.
-    destruct H.
-     unfold interp.
-     unfold interp in H,H0.
-     now rewrite H,H0.
-  - intro.
-    split;
-
-    unfold interp in H;
-      symmetry in  H;
-      apply Bool.andb_true_eq in H;
-      destruct H;
-      unfold interp;
-      symmetry;
-      assumption.
-      
-Qed.
-
-Lemma lor_interp_interp: forall p1 p2 V, interp V p1=true \/ interp V p2=true <-> interp V (lor p1 p2)=true.
-Proof.
-  intros.
-  split.
-  - intro.
-    destruct H.
-     unfold interp.
-     unfold interp in H.
-     rewrite H. reflexivity.
-     unfold interp.
-     unfold interp in H.
-     rewrite H. Search orb. apply Bool.orb_true_r.
-  - intro.
-
+  split;
+    intros;
     unfold interp in H.
-    Search orb.
-    apply Bool.orb_prop in H.
-   
-      unfold interp;
-      assumption.
-      
-Qed.
-
-
-Lemma mapsto_interp_interp: forall p1 p2 V, interp V p1=false \/ interp V p2=true <-> interp V (mapsto p1 p2)=true.
-Proof.
-  intros.
-  split.
-  - intro.
+  - (* -> *)
     destruct H.
-     unfold interp.
-     unfold interp in H.
-     rewrite H. reflexivity.
-     unfold interp.
-     unfold interp in H.
-     rewrite H. apply Bool.orb_true_r.
-  - intro.
-
-    unfold interp in H.
-    Search orb.
-    apply Bool.orb_prop in H.
-    destruct H.
-    + left.
-      
-      unfold interp.
-      Search negb.
-      now apply Bool.negb_true_iff.
-    + right.
-      unfold interp.
-      assumption.
-Qed.
-
-
-
-Lemma not_interp_interp: forall p V, interp V p=false  <-> interp V (not p)=true.
-Proof.
-  intros.
-  split.
-  - intro.
-     unfold interp.
-     unfold interp in H.
-     rewrite H. reflexivity.
-  - intro.
-
-    unfold interp in H.
-
+    (* has interp p1 = true, interp p2 = true*)
     unfold interp.
-    now apply Bool.negb_true_iff.
+    unfold interp in H0.
+    now rewrite H,H0.
+  - (* <- *)
+    split;(*proofs for both sub-forms are same*)
+    split_andb_ture H;
+    assumption.
+Qed.
+
+Lemma split_interp_lor: forall p1 p2 V, interp V p1=true \/ interp V p2=true <-> interp V (lor p1 p2)=true.
+Proof.
+  split;
+    intros;
+    unfold interp in H.
+  - (* -> *)
+    destruct H;
+      unfold interp;
+      rewrite H.
+    + reflexivity. (*has true || x = true*)
+    + apply orb_true_r. (*has x || true = true, need a lemma*)
+  - (* -> *)
+    apply orb_prop in H. (*convert from a || b = true -> a=true \/ b =true*)
+    assumption.
+Qed.
+
+
+Lemma split_interp_mapsto: forall p1 p2 V, interp V p1=false \/ interp V p2=true <-> interp V (mapsto p1 p2)=true.
+Proof.
+  split;
+    intros;
+    unfold interp in H.
+  - (* -> *) (*same as lor, since mapsto x y = lor (not x) y*)
+    destruct H;
+      unfold interp;
+      rewrite H.
+    + reflexivity.
+    + apply orb_true_r.
+  - (* <- *)
+    apply orb_prop in H.
+    destruct H.
+    + left. (*handle not*)
+      apply negb_true_iff. (*a= false -> negb a =true*)
+      assumption.
+    + right.
+      assumption.
+Qed.
+
+
+Lemma split_interp_not: forall p V, interp V p=false  <-> interp V (not p)=true.
+Proof.
+  split;
+    intros;
+    unfold interp in H;
+    unfold interp.
+  - (* -> *)   
+    rewrite H.
+    reflexivity.
+  - (* <- *)
+    unfold interp.
+    apply negb_true_iff. (*same as mapsto*)
+    assumption.
 Qed.
